SSA/Projects/RISCV/RV64InstrRewrite.lean
@@ -7,8 +7,30 @@ import SSA.Core.Util
 
 open MLIR AST in
 
---typing test
+-- additional lemmas introduced for the proofs.
 
+--@[simp] --> to do: fix it
+theorem get_cons_succ0 {A : α → Type*} {a : α} {as : List α}
+  (e : A a) (vec : HVector A as) (i : Fin as.length) :
+  (e::ₕvec).get i.succ = vec.get i := by rfl -- extracting the i succ elem is like extracting the i elem from the remaining list
+
+--@[simp]
+--theorem get_cons_succ {A : α → Type*} {a : α} {as : List α}
+  --(e : A a) (vec : HVector A as) (i : Fin (as.length)):
+  --((e::ₕvec)).get ((i + 1)) = ((vec) : HVector A (as)).get (i : Fin (as.length))  := by rfl -- extracting the i succ elem is like extracting the i elem from the remaining list
+
+--@[simp]
+theorem get_cons_1 {A : α → Type*} {a b: α} {as : List α}
+  (e : A a) (f : A b) (vec : HVector A as)  :
+--((e::ₕ (f ::ₕ vec)) : HVector A (a :: b :: as)).get ⟨1, by simp⟩ = f := by rfl -- extracting the i succ elem is like extracting the i elem from the remaining list
+  ((e::ₕ (f ::ₕ vec)) : HVector A (a :: b :: as)).get (1 : Fin (as.length + 2)) = f := by rfl -- extracting the i succ elem is like extracting the i elem from the remaining list
+
+
+-- modelled the same rewrites done on the llvm ir level in assembly
+--next goal:
+  ---extract the llvm based on bitvectors
+
+-- add rd rs1 rs1 <-> slli rd rs1 $1
 theorem addTwice_eq_shiftLeftOnce :
   [RV64_com| {
   ^entry (%0: !i64 ):
@@ -18,91 +40,342 @@ theorem addTwice_eq_shiftLeftOnce :
   [RV64_com| {
   ^entry (%0 : !i64 ):
     %1 = "RV64.slli" (%0) { shamt = 1 : !i64 } : ( !i64) -> (!i64)
-    "return" (%1) : ( !i64 ) -> ()
+    "return" (%1) : (!i64 ) -> ()
 }].denote := by
   funext Γv
-  simp_peephole at Γv
+  simp_peephole at Γv -- simplifies a :: in the resolve what values variables map to --> directly TV v for some variable v which gives me the valuation of the varialbe of ty in cotext T
   simp
   unfold RV64.RTYPE_pure64_RISCV_ADD RV64.SHIFTIOP_pure64_RISCV_SLLI
   bv_decide
 
-theorem bitvec : e + e + (e + e) = BitVec.mul e 4#64 := by bv_decide
 
-theorem addFourth_eq_shiftLeftTwice :
-  [RV64_com| {
-  ^entry (%0: !i64 ):
-  %1 = "RV64.add" (%0, %0) : (!i64, !i64) -> (!i64)
-  %2 = "RV64.add" (%1, %1) : (!i64, !i64) -> (!i64)
-  "return" (%2) : (!i64) -> ()
+/-  add rd rs1 rs1
+    add rd rd rd
+    ==
+    slli rd rs1 $2
+-/
+
+  theorem addFourth_eq_shiftLeftTwice :
+    [RV64_com| {
+    ^entry (%0: !i64 ):
+    %1 = "RV64.add" (%0, %0) : (!i64, !i64) -> (!i64)
+    %2 = "RV64.add" (%1, %1) : (!i64, !i64) -> (!i64)
+    "return" (%2) : (!i64) -> ()
+    }].denote =
+    [RV64_com| {
+    ^entry (%0 : !i64 ):
+      %1 = "RV64.slli" (%0) { shamt = 2 : !i64 } : ( !i64) -> (!i64)
+      "return" (%1) : ( !i64 ) -> ()
+  }].denote := by
+    funext Γv
+    simp_peephole at Γv
+    simp
+    unfold RV64.RTYPE_pure64_RISCV_ADD RV64.SHIFTIOP_pure64_RISCV_SLLI
+    simp [BitVec.add_eq, BitVec.toNat_ofNat, Nat.reducePow, Nat.reduceMod, BitVec.shiftLeft_eq]
+    intro e
+    show @Eq (BitVec _) (e + e + (e + e)) (e <<< 2) -- used to help Lean to discover the type of the operation
+    --show (e + e + (e + e)) = (e <<< 2) also works
+    bv_decide
+
+
+/-  and rd rs1 $0
+    ==
+    $0
+-/
+  theorem andZero_eq_zero :
+    [RV64_com| {
+    ^entry (%0: !i64 ):
+      %1 = "RV64.const" () { val = 0 : !i64  } : ( !i64 ) -> (!i64)
+      %2 = "RV64.and" (%0, %1) : ( !i64, !i64 ) -> (!i64)
+      "return" (%2) : ( !i64) -> ()
   }].denote =
-  [RV64_com| {
-  ^entry (%0 : !i64 ):
-    %1 = "RV64.slli" (%0) { shamt = 2 : !i64 } : ( !i64) -> (!i64)
-    "return" (%1) : ( !i64 ) -> ()
-}].denote := by
+    [RV64_com| {
+    ^entry (%0 : !i64 ):
+      %1 = "RV64.const" () { val = 0 : !i64  } : ( !i64 ) -> (!i64)
+      "return" (%1) : ( !i64 ) -> ()
+  }].denote := by
+      funext Γv
+      simp_peephole at Γv
+      simp
+      unfold RV64.RTYPE_pure64_RISCV_AND RV64.const_func
+      bv_decide
+
+/-  mul rd rs1 $1
+    ==
+    slli rd rs1 $0
+-/
+  theorem mulOne_eq_shiftZero :
+    [RV64_com| {
+    ^entry (%0: !i64 ):
+      %1 = "RV64.const" () { val = 1 : !i64  } : (!i64) -> (!i64)
+      %2 = "RV64.mulu" (%0, %1) : ( !i64, !i64 ) -> (!i64)
+      "return" (%2) : ( !i64 ) -> ()
+  }].denote =
+    [RV64_com| {
+    ^entry (%0 : !i64 ):
+      %1 = "RV64.slli" (%0) { shamt = 0 : !i64 } : ( !i64) -> (!i64)
+      "return" (%1) : ( !i64 ) -> ()
+  }].denote := by
+      funext Γv
+      simp_peephole at Γv
+      simp
+      unfold RV64.MUL_pure64_fff RV64.SHIFTIOP_pure64_RISCV_SLLI RV64.const_func
+      intro e
+      show @Eq (BitVec _) _ _
+      simp [get_cons_1]
+      bv_decide
+
+/-
+    sub rd rs1 rs1
+    xor rd rd rs2
+    return rd
+    ==
+    return rs2
+-/
+  theorem xor_sub : -- taken from the peephole rewrite
+    [RV64_com| {
+      ^entry (%r1: !i64, %r2: !i64 ) :
+        %0 = "RV64.sub" (%r1, %r1) : (!i64,!i64 ) -> (!i64)
+        %1 = "RV64.xor" (%0,%r2) : (!i64,!i64 ) -> (!i64)
+      "return" (%1) : (!i64 ) -> ()
+    }].denote =
+    [RV64_com| {
+      ^entry (%r1: !i64, %r2: !i64 ) :
+       "return" (%r2) : (!i64 ) -> ()
+      }].denote := by
+      funext Γv
+      simp_peephole at Γv
+      simp only [Fin.isValue, HVector.cons_get_zero]
+      intros e s
+      unfold RV64.RTYPE_pure64_RISCV_XOR RV64.RTYPE_pure64_RISCV_SUB
+      show @Eq (BitVec 64) _ _
+      --show @Eq (BitVec 64) ((s.sub s).xor e) e
+      bv_decide
+
+
+/-  xor rd x1 x1
+    return rd
+    ==
+    return $0
+-/
+def RISCVEg1 := [RV64_com| {
+  ^entry (%x1: !i64):
+    %1 = "RV64.xor" (%x1, %x1) : (!i64, !i64) -> (!i64)
+    "return" (%1) : (!i64) -> ()
+}].denote
+
+def RISCVZero := [RV64_com| {
+  ^entry (%x1: !i64):
+    %1 =  "RV64.const" () { val = 0 : !i64  } : (!i64) -> (!i64)
+    "return" (%1) : (!i64) -> ()
+}].denote
+
+theorem xor_eq_zero :
+  RISCVEg1 = RISCVZero := by
+  unfold RISCVEg1 RISCVZero
   funext Γv
   simp_peephole at Γv
-  simp
-  unfold RV64.RTYPE_pure64_RISCV_ADD RV64.SHIFTIOP_pure64_RISCV_SLLI
-  simp [BitVec.add_eq, BitVec.toNat_ofNat, Nat.reducePow, Nat.reduceMod, BitVec.shiftLeft_eq]
-  intro
-  rw [bitvec]
+  intro e
+  unfold RV64.RTYPE_pure64_RISCV_XOR RV64.const_func
+  rw[HVector.cons_get_zero]
+  show @Eq (BitVec 64) _ _
   bv_decide
 
-theorem andZero_eq_zero :
-  [RV64_com| {
-  ^entry (%0: !i64 ):
-    %1 = "RV64.const" (%0) { val = 0 : !i64  } : ( !i64 ) -> (!i64)
-    %2 = "RV64.and" (%0, %1) : ( !i64, !i64 ) -> (!i64)
-    "return" (%2) : ( !i64) -> ()
-}].denote =
-  [RV64_com| {
-  ^entry (%0 : !i64 ):
-     %1 = "RV64.const" (%0) { val = 0 : !i64  } : ( !i64 ) -> (!i64)
-    "return" (%1) : ( !i64 ) -> ()
-}].denote := by
-    funext Γv
-    simp_peephole at Γv
-    simp
-    unfold RV64.RTYPE_pure64_RISCV_AND RV64.const_func
-    bv_decide
 
-
-theorem t2 :
-  [RV64_com| {
-  ^entry (%0: !i64 ):
-    %1 = "RV64.const" (%0) { val = 1 : !i64  } : ( !i64 ) -> (!i64)
-    %2 = "RV64.mul" (%0, %1)  { high = 0 : !i64 , s1 = 0 : !i64, s2 = 0 : !i64  } : ( !i64, !i64 ) -> (!i64)
-    "return" (%2) : ( !i64 ) -> ()
-}].denote =
-  [RV64_com| {
-  ^entry (%0 : !i64 ):
-    %1 = "RV64.slli" (%0) { shamt = 0 : !i64 } : ( !i64) -> (!i64)
-    "return" (%1) : ( !i64 ) -> ()
-}].denote := by
-    funext Γv
-    simp_peephole at Γv
-    simp
-    unfold RV64.MUL_pure64_fff RV64.SHIFTIOP_pure64_RISCV_SLLI RV64.const_func
-    intro
-    simp
-    bv_decide
-
-
-
-
+/-
+-/
 def RISCVEg25 := [RV64_com| {
   ^entry (%0: !i64 ):
-    %1 = "RV64.const" (%0) { val = 2 : !i64  } : ( !i64 ) -> (!i64)
-    %2 = "RV64.mul" (%0, %1)  { high = 0 : !i64 , s1 = 0 : !i64, s2 = 0 : !i64  } : ( !i64, !i64 ) -> (!i64)
+    %1 = "RV64.const" () { val = 2 : !i64  } : ( !i64 ) -> (!i64)
+    %2 = "RV64.mulu" (%0, %1)  : ( !i64, !i64 ) -> (!i64)
     "return" (%2) : ( !i64, !i64 ) -> ()
-}]
+}].denote
 
 def RISCVEg26 := [RV64_com| {
   ^entry (%0: !i64, %1: !i64 ):
-    %2 = "RV64.mul" (%0, %1)  { high = 0 : !i64 , s1 = 0 : !i64, s2 = 0 : !i64  } : ( !i64, !i64 ) -> (!i64)
+    %2 = "RV64.mulu" (%0, %1)  : ( !i64, !i64 ) -> (!i64)
     "return" (%2) : ( !i64, !i64 ) -> ()
-}]
+}].denote
+
+
+
+-- section where I start to rewrite things from alive
+
+/-  add rd rs1 rs1
+    ==
+    slli rd rs1 1
+-/
+def RISCVE_AddSub_src := [RV64_com| {
+  ^entry (%0: !i64 ):
+    %v1 = "RV64.add" (%0, %0) : ( !i64, !i64 ) -> (!i64)
+    "return" (%v1) : ( !i64, !i64 ) -> ()
+}].denote
+
+def RISCVE_AddSub_opt := [RV64_com| {
+  ^entry (%0: !i64 ):
+    %v1 = "RV64.slli" (%0) { shamt = 1 : !i64 } : ( !i64) -> (!i64)
+    "return" (%v1) : ( !i64, !i64 ) -> ()
+}].denote
+
+theorem RISCV64_AddSub : RISCVE_AddSub_src = RISCVE_AddSub_opt := by
+  unfold RISCVE_AddSub_src RISCVE_AddSub_opt
+  funext Γv
+  simp_peephole at Γv
+  intro e
+  unfold RV64.RTYPE_pure64_RISCV_ADD RV64.SHIFTIOP_pure64_RISCV_SLLI
+  rw [HVector.cons_get_zero, HVector.cons_get_zero]
+  bv_decide
+
+
+/-  sub rd1 v1 $0 -- -a
+    add rd2 rd1 b -- (-a) + b
+    return rd2 -- (-a) + b
+    ==
+    sub rd b v1
+-/
+
+def RISCVE_AddSub1164_src := [RV64_com| {
+  ^entry (%a: !i64, %b: !i64 ):
+    %v1 = "RV64.const" () { val = 0 : !i64  } : ( !i64 ) -> (!i64)
+    %v2 = "RV64.sub" (%a, %v1 ) : ( !i64, !i64 ) -> (!i64)
+    %v3 = "RV64.add" (%v2 , %b ) : ( !i64, !i64 ) -> (!i64)
+    "return" (%v3) : (!i64, !i64) -> ()
+}].denote
+
+def RISCVE_AddSub1164_opt := [RV64_com| {
+  ^entry (%a: !i64, %b: !i64 ):
+    %v1 = "RV64.sub" (%a, %b) : ( !i64, !i64 ) -> (!i64) -- b - a
+    "return" (%v1) : (!i64, !i64) -> ()
+}].denote
+
+theorem RISCV64_AddSub1164 :
+  RISCVE_AddSub1164_src = RISCVE_AddSub1164_opt := by
+  unfold RISCVE_AddSub1164_opt RISCVE_AddSub1164_src
+  funext Γv
+  simp_peephole at Γv
+  intro e1 e2
+  unfold RV64.RTYPE_pure64_RISCV_ADD RV64.RTYPE_pure64_RISCV_SUB RV64.const_func
+  simp [HVector.cons_get_zero]
+  bv_decide
+
+/-  sub rd1 v1 $0 -- -a
+    add rd2 rd1 b -- (-a) + b
+    return rd2 -- (-a) + b
+    ==
+    sub rd b v1
+-/
+def RISCVE_AddSub1164_src2 := [RV64_com| {
+  ^entry (%a: !i64, %b: !i64 ):
+    %v1 = "RV64.const" () { val = 0 : !i64  } : ( !i64 ) -> (!i64)
+    %v2 = "RV64.sub" (%a, %v1 ) : ( !i64, !i64 ) -> (!i64) -- 0-a
+    %v3 = "RV64.add" (%b, %v2 ) : ( !i64, !i64 ) -> (!i64) -- b - a
+    "return" (%v3) : (!i64, !i64) -> ()
+}].denote
+
+
+def RISCVE_AddSub1164_opt2 := [RV64_com| {
+  ^entry (%a: !i64, %b: !i64 ):
+    %v1 = "RV64.const" () { val = 0 : !i64  } : ( !i64 ) -> (!i64) -- 0
+    %v2 = "RV64.sub" (%a, %v1 ) : ( !i64, !i64 ) -> (!i64) -- 0 - a basically dead code
+    %v3 = "RV64.sub" ( %a ,  %b ) : ( !i64, !i64 ) -> (!i64) -- b- a
+    "return" (%v3) : (!i64, !i64) -> ()
+}].denote
+
+theorem RISCV64_AddSub1164_2 :
+  RISCVE_AddSub1164_src2 = RISCVE_AddSub1164_opt2 := by
+  unfold RISCVE_AddSub1164_opt2 RISCVE_AddSub1164_src2
+  funext Γv
+  simp_peephole at Γv
+  intro e1 e2
+  unfold RV64.RTYPE_pure64_RISCV_SUB RV64.const_func RV64.RTYPE_pure64_RISCV_ADD
+  simp [HVector.cons_get_zero]
+  show @Eq (BitVec 64) _ _
+  bv_decide
+
+
+
+def RV64_DivRemOfSelect_src := [RV64_com| {
+  ^entry (%c: !i64, %y: !i64, %x: !i64):
+    %c0 = "RV64.const" () { val = 0 : !i64  } : ( !i64 ) -> (!i64) -- 0
+    %v1 = "RV64.czero.nez" ( %c0, %y ) : ( !i64, !i64 ) -> (!i64) -- if c0 is zero then y else 0 --> fixed to y
+    %v2 = "RV64.divu" ( %v1, %x ) : ( !i64, !i64 ) -> (!i64) -- x / v1
+    "return" (%v2) : (!i64, !i64,!i64 ) -> ()
+}].denote
+
+def RV64_DivRemOfSelect_opt := [RV64_com| {
+  ^entry (%c: !i64, %y: !i64, %x: !i64):
+    %v1 = "RV64.divu" ( %y, %x )  : ( !i64, !i64 ) -> (!i64) -- x / y
+    "return" (%v1) : (!i64) -> ()
+}].denote
+
+theorem RV64_DivRemOfSelect :
+ RV64_DivRemOfSelect_src = RV64_DivRemOfSelect_opt :=
+  by
+  unfold RV64_DivRemOfSelect_src RV64_DivRemOfSelect_opt
+  funext Γv
+  simp_peephole at Γv
+  simp
+  intro e1 e2
+  unfold RV64.ZICOND_RTYPE_pure64_RISCV_RISCV_CZERO_NEZ RV64.const_func RV64.DIV_pure64_unsigned
+  simp only [Nat.sub_zero, Nat.reduceAdd, BitVec.zero_eq, ↓reduceIte, BitVec.extractLsb_toNat,
+    Nat.shiftRight_zero, Nat.reducePow, Int.ofNat_eq_coe, Int.ofNat_emod, Nat.cast_ofNat,
+    Int.reduceNeg, Int.ofNat_toNat]
+
+
+def RISCVEgDCE_src := [RV64_com| {
+  ^entry (%x1: !i64):
+    %0 = "RV64.add" (%x1, %x1) : (!i64, !i64) -> (!i64) -- dead code not used
+    %1 = "RV64.add" (%x1, %x1) : (!i64, !i64) -> (!i64)
+    "return" (%1) : (!i64) -> ()
+}].denote
+
+def RISCVDCE_opt := [RV64_com| {
+  ^entry (%x1: !i64):
+    %0 = "RV64.add" (%x1, %x1) : (!i64, !i64) -> (!i64)
+    "return" (%0) : (!i64) -> ()
+}].denote
+
+theorem DCE1 :
+  RISCVEgDCE_src = RISCVDCE_opt := by
+    unfold RISCVEgDCE_src RISCVDCE_opt
+    funext Γv
+    simp_peephole at Γv
+
+
+/-
+%r = sdiv 1, %X
+  =>
+%inc = add %X, 1
+%c = icmp ult %inc, 3
+%r = select %c, %X, 0
+-/
+
+
+/-
+def alive_DivRemOfSelect_src (w : Nat) :=
+  [llvm(w)| {
+  ^bb0(%c: i1, %y : _, %x : _):
+    %c0 = llvm.mlir.constant(0) : _
+    %v1 = llvm.select %c, %y, %c0
+    %v2 = llvm.udiv %x,  %v1
+    llvm.return %v2
+  }]
+def alive_DivRemOfSelect_tgt (w : Nat) :=
+  [llvm(w)| {
+  ^bb0(%c: i1, %y : _, %x : _):
+    %v1 = llvm.udiv %x, %y
+    llvm.return %v1
+  }]
+-/
+
+/-
+%r = sdiv 1, %X
+  =>
+%inc = add %X, 1
+%c = icmp ult %inc, 3
+%r = select %c, %X, 0
+-/
+
 
 /-
   ^entry(%0 : ToyRegion.Ty.int):
