SSA/Projects/InstCombine/PaperExamples.lean
@@ -40,16 +40,6 @@ info: 'AlivePaperExamples.shift_mul' depends on axioms: [propext, Quot.sound]
 #guard_msgs in #print axioms shift_mul
 
 -- Example proof of xor + sub, this is automatically closed by automation.
-theorem xor_sub :
-    [llvm(w)| {
-  ^bb0(%X : _, %Y : _):
-    %v1 = llvm.sub %X, %X
-    %r = llvm.xor %v1, %Y
-    llvm.return %r
-  }] ⊑  [llvm(w)| {
-  ^bb0(%X : _, %Y : _):
-    llvm.return %Y
-  }] := by
     simp_alive_peephole
     alive_auto
 
