SSA/Projects/RISCV/LLVMtoRISCV.lean
@@ -1,0 +1,352 @@
+import SSA.Projects.RISCV.RV64
+import SSA.Projects.InstCombine.LLVM.Semantics
+import SSA.Projects.InstCombine.LLVM.PrettyEDSL
+import SSA.Projects.InstCombine.Refinement
+import SSA.Projects.InstCombine.Tactic
+import SSA.Projects.InstCombine.TacticAuto
+import SSA.Projects.InstCombine.Base
+import SSA.Projects.InstCombine.ForLean
+import Lean
+import Mathlib.Tactic.Ring
+import SSA.Projects.InstCombine.ForLean
+import SSA.Projects.InstCombine.LLVM.EDSL
+import SSA.Experimental.Bits.Fast.Reflect
+import SSA.Experimental.Bits.Fast.MBA
+import SSA.Experimental.Bits.FastCopy.Reflect
+import SSA.Experimental.Bits.AutoStructs.Tactic
+import SSA.Experimental.Bits.AutoStructs.ForLean
+import Std.Tactic.BVDecide
+import SSA.Core.Tactic.TacBench
+import Leanwuzla
+/-
+def eg1 :=
+  [llvm(64)| {
+^bb0(%X : _, %Y : _):
+      %v1 = llvm.and %X, %Y
+      %v2 = llvm.or %X, %Y
+      %v3 = llvm.add %v1, %v2
+      llvm.return %v3
+  }].denote
+-/
+
+
+def eg22 :=
+  [RV64_com| {
+    ^entry (%X: !i64, %Y: !i64):
+    %v1 = "RV64.add" (%X, %Y) : (!i64, !i64) -> (!i64)
+    "return" (%v1) : (!i64, !i64) -> ()
+  }].denote
+
+
+
+def eg21_b :=
+  [llvm(64)| {
+^bb0(%X : i64, %Y : i64):
+      %v1 = llvm.add %Y, %X : i64
+      llvm.return %v1 : i64
+  }]
+
+#check eg21_b --(Γv : ((Ctxt.snoc [] toRISCV.Ty.bv).snoc toRISCV.Ty.bv).Valuation)
+def lh_llvm : (HVector TyDenote.toType [InstCombine.Ty.bitvec 64,InstCombine.Ty.bitvec 64]) :=
+          HVector.cons (some (BitVec.ofNat 64 20)) <| HVector.cons (some (BitVec.ofNat 64 2)) .nil
+-- creating an HVector but specifying the types bc Lean can't just infer it
+#check lh -- dependetly typed HVector
+
+def test_add_llvm : Option (BitVec 64) := eg21_b.denote (Ctxt.Valuation.ofHVector lh_llvm)
+#eval test_add_llvm
+
+
+theorem add_llvm_eq_bc :
+  eg21_b.denote (Ctxt.Valuation.ofHVector lh_llvm) = some x →
+    x = (BitVec.add (BitVec.ofNat 64 20) (BitVec.ofNat 64 2))
+  := by
+  unfold eg21_b lh_llvm
+  simp_alive_meta
+  simp_peephole [InstCombine.Op.denote,HVector.get,HVector.get, LLVM.add]
+  simp [HVector.cons_get_zero]
+  simp_alive_undef
+  intro h
+  injection h with h₁
+  rw [← h₁]
+  bv_decide
+
+def lh_riscv : HVector TyDenote.toType [toRISCV.Ty.bv,toRISCV.Ty.bv ] :=
+  HVector.cons ((BitVec.ofNat 64 20)) <| HVector.cons ( (BitVec.ofNat 64 2)) .nil -- hvector from which we will create the valuation
+def test_add_riscv : BitVec 64 := eg22 (Ctxt.Valuation.ofHVector lh_riscv)
+#eval test_add_riscv
+
+-- managed the proof the bit vec domain
+theorem add_riscv_eq_bv :
+  eg22 (Ctxt.Valuation.ofHVector lh_riscv) = BitVec.add (BitVec.ofNat 64 20) (BitVec.ofNat 64 2)
+  := by
+  unfold eg22 lh_riscv
+  simp_peephole
+  unfold RV64.RTYPE_pure64_RISCV_ADD
+  simp [HVector.cons_get_zero]
+
+-- first steps
+-- example where I still modell both contexts explictily
+theorem translation_add :
+    eg21_b.denote (Ctxt.Valuation.ofHVector lh_llvm) = some x →
+      x = eg22 (Ctxt.Valuation.ofHVector lh_riscv) := by
+    rw [add_riscv_eq_bv]
+    apply add_llvm_eq_bc
+
+-- diffrent step where I attempt to have only one proof
+theorem translation_add_combined :
+    eg21_b.denote (Ctxt.Valuation.ofHVector lh_llvm) = some x →
+      x = eg22 (Ctxt.Valuation.ofHVector lh_riscv) := by
+    unfold eg22 lh_riscv eg21_b lh_llvm
+    simp_alive_meta
+    simp_peephole [InstCombine.Op.denote,HVector.get,HVector.get, LLVM.add]
+    unfold RV64.RTYPE_pure64_RISCV_ADD
+    simp [HVector.cons_get_zero]
+    simp_alive_undef
+    intro h
+    injection h with h₁
+    rw [← h₁]
+    bv_decide
+
+-- attempt 3 where I try to have a universal context
+--def contextMap
+--def contextRefine :
+  def ADD_LLVM_BIG_CONTEXT :=
+    [llvm(64)| {
+^bb0(%X : i64, %Y : i64, %Z : i64, %W : i64 ):
+      %v1 = llvm.add %Y, %X : i64
+      llvm.return %v1 : i64
+  }]
+def lh_llvm_big : (HVector TyDenote.toType [InstCombine.Ty.bitvec 64,InstCombine.Ty.bitvec 64,InstCombine.Ty.bitvec 64,InstCombine.Ty.bitvec 64 ]) :=
+          HVector.cons (some (BitVec.ofNat 64 20)) <| HVector.cons (some (BitVec.ofNat 64 2)) <| HVector.cons (some (BitVec.ofNat 64 20)) <| HVector.cons (some (BitVec.ofNat 64 2)) .nil
+
+theorem larger_context :
+  ADD_LLVM_BIG_CONTEXT.denote (Ctxt.Valuation.ofHVector lh_llvm_big) = some x →
+    x = eg22 (Ctxt.Valuation.ofHVector lh_riscv)
+  := by
+  unfold ADD_LLVM_BIG_CONTEXT eg22 lh_llvm_big lh_riscv
+  simp_alive_meta
+  simp_peephole [InstCombine.Op.denote,HVector.get,HVector.get, LLVM.add]
+  simp [HVector.cons_get_zero]
+  simp_alive_undef
+  unfold RV64.RTYPE_pure64_RISCV_ADD
+  intro h
+  injection h with h₁
+  rw [← h₁]
+  bv_decide
+
+
+ theorem testLLVMOnly1 :
+  eg21_a ⊑  eg21_b := by
+  unfold eg21_a eg21_b
+  simp_alive_meta
+  intros Γv
+  simp_peephole [InstCombine.Op.denote] at Γv
+  simp (config := {failIfUnchanged := false}) only [
+            InstCombine.Op.denote, HVector.getN, HVector.get,
+            beq_self_eq_true, Option.isSome_some, HVector.cons_get_zero
+          ]
+  simp (config := {failIfUnchanged := false }) only [Nat.cast_ofNat,
+          Nat.cast_one, Int.reduceNegSucc, Int.reduceNeg]
+  simp_alive_undef
+  simp_alive_case_bash'
+  . intro x1 x2
+    bv_decide
+
+
+#check TyDenote.toType
+--def Γv : HVector (BitVec 64) 2 := HVector.cons x1 (HVector.cons x2 HVector.nil)
+/-
+
+((InstcombineTransformDialect.MOp.instantiateCom ⟨[sorry], ⋯⟩).mapTy <$>
+      (Ctxt.snoc [] (InstCombine.MTy.bitvec 64)).snoc (InstCombine.MTy.bitvec 64)).Valuation
+
+-/
+def lh : HVector TyDenote.toType [InstCombine.Ty.bitvec 64,InstCombine.Ty.bitvec 64]
+  :=  HVector.cons (some (BitVec.ofNat 64 0)) <| HVector.cons (some (BitVec.ofNat 64 2)) .nil
+
+
+
+
+
+theorem testLLVMOnly_explicitContext :
+  let Γv := (Ctxt.Valuation.ofHVector lh)
+  eg21_a.denote Γv  =  eg21_b.denote Γv := by
+  unfold eg21_a eg21_b
+  sorry
+  --intro Γv
+  --simp_alive_meta
+  --simp_peephole [InstCombine.Op.denote]
+  --simp [InstCombine.Op.denote,HVector.getN,HVector.get]
+  --simp_alive_undef
+  --simp_alive_case_bash'
+  --. intro x1 x2
+    --apply congrArg some
+    --bv_decide
+
+
+theorem testLLVMOnly :
+  eg21.denote Γv  =  eg21_b.denote  Γv := by
+  unfold eg21 eg21_b
+  simp_alive_meta
+  simp_peephole [InstCombine.Op.denote] at Γv
+  simp [InstCombine.Op.denote,HVector.getN,HVector.get]
+  simp_alive_undef
+  simp_alive_case_bash'
+  . intro x1 x2
+    apply congrArg some
+    bv_decide
+
+  --simp_alive_meta
+  /-
+
+
+((InstcombineTransformDialect.MOp.instantiateCom ⟨[sorry], ⋯⟩).mapTy <$>
+      (Ctxt.snoc [] (InstCombine.MTy.bitvec 64)).snoc (InstCombine.MTy.bitvec 64)).Valuation
+
+
+
+
+
+
+
+
+  ((InstcombineTransformDialect.MOp.instantiateCom ⟨[sorry], ⋯⟩).mapTy <$>
+    (Ctxt.snoc [] (InstCombine.MTy.bitvec 64)).snoc (InstCombine.MTy.bitvec 64)).Valuation
+
+def lh54 : HVector TyDenote.toType [toRISCV.Ty.bv, toRISCV.Ty.bv ]
+  := HVector.cons (BitVec.ofNat 64 8) <| HVector.cons (BitVec.ofNat 64 1) .nil
+
+def test_ror : BitVec 64 := RISCVEg54.denote (Ctxt.Valuation.ofHVector lh54)
+#eval test_ror
+
+  -/
+
+  --simp [Com.changeDialect_ret,
+        --Com.changeDialect_var, Expr.changeDialect]
+  --simp_alive_meta
+  --simp_alive_peephole
+  --simp_alive_undef
+  --simp_alive_case_bash
+  --. bv_decide
+
+
+
+def LLVMCtxt := Ctxt InstCombine.Ty
+def RISCVCtxt := Ctxt toRISCV.Ty
+
+
+def CtxtRefines (Γ : LLVMCtxt) (Δ : RISCVCtxt) : Type := -- defining how to the types are mapped between the two contexts
+  (Δ.Var .bv) → Γ.Var (.bitvec 64)
+
+#print CtxtRefines
+
+--def V₁:= (Ctxt.Valuation.ofHVector lh_llvm)
+--def V₂:= (Ctxt.Valuation.ofHVector lh_riscv)
+
+
+
+
+
+
+structure ValuationRefines {Γ : LLVMCtxt} {Δ : RISCVCtxt} (V₁ : Γ.Valuation) (V₂ : Δ.Valuation) where
+  ctxtRefines : CtxtRefines Γ Δ -- defining how to values should be mapped, challenge; llvm type is option bc of UB
+  val_refines : ∀ (v : Δ.Var .bv) (x : BitVec 64), V₁ (ctxtRefines v) = some x → V₂ v = x --if the llvm variable has a some value we have the riscv value given
+
+theorem see_LLVM_concrete3 V₁ V₂ (h : ValuationRefines V₁ V₂) : -- have the assumptions given by Valuation Refines
+    eg21_b.denote V₁ = some x → eg22 V₂ = x := by -- llvm to risc-v
+
+
+
+
+
+
+
+
+
+
+
+#check lh_llvm
+#check lh_riscv
+#check CtxtRefines
+#check Ctxt toRISCV.Ty
+
+
+theorem see_LLVM_concrete V₁ V₂ (h : ValuationRefines V₁ V₂) :
+    eg21_b.denote V₁ = some x → eg22 V₂ = x := by
+  unfold eg21_b eg22
+  let ⟨ctxtRef, val_ref⟩ := h
+  simp_alive_meta
+  simp_peephole [InstCombine.Op.denote,HVector.get,HVector.get, LLVM.add]
+  unfold RV64.RTYPE_pure64_RISCV_ADD
+  simp [HVector.cons_get_zero]
+  simp_alive_undef
+
+  --intro h
+
+
+
+
+
+
+
+
+
+
+
+
+
+  --simp [V₁]
+
+
+
+
+
+/-
+theorem translation_add_combined :
+    eg21_b.denote (Ctxt.Valuation.ofHVector lh_llvm) = some x →
+      x = eg22 (Ctxt.Valuation.ofHVector lh_riscv) := by
+    unfold eg22 lh_riscv eg21_b lh_llvm
+    simp_alive_meta
+    simp_peephole [InstCombine.Op.denote,HVector.get,HVector.get, LLVM.add]
+    unfold RV64.RTYPE_pure64_RISCV_ADD
+    simp [HVector.cons_get_zero]
+    simp_alive_undef
+    intro h
+    injection h with h₁
+    rw [← h₁]
+    bv_decide
+-/
+
+
+theorem see_LLVM (V₁) (V₂) (h : ValuationRefines V₁ V₂) :
+  eg21_b.denote V₁ = some x → eg22 V₂ = x := by
+  unfold eg21_b eg22
+
+
+
+
+
+theorem see_LLVM1 (V₁) (V₂) (h : ValuationRefines V₁ V₂) :
+    ∃ x, eg21_b.denote V₁ = some x → eg22 V₂ = x := by
+  unfold eg21 eg22
+  sorry
+
+
+
+
+
+  --simp only [Com.denote]
+  simp_alive_meta
+  simp_peephole
+  --simp [DialectDenote.denote]
+  let ⟨ctxtRef, val_ref⟩ := h
+  let X_RV := Ctxt.Var.last [] toRISCV.Ty.bv
+  let Y_RV := Ctxt.Var.last [toRISCV.Ty.bv] toRISCV.Ty.bv
+  let X_LL := h.ctxtRefines X_RV
+  let Y_LL := h.ctxtRefines Y_RV
+  cases V₁ X_LL with --none or some
+  | none  => sorry
+  | some x₁ => -- resolving x first
+    cases V₁ Y_LL with
+      | none => sorry
+      | some x₂ =>
