SSA/Projects/RISCV/translationNaive.lean
@@ -1,0 +1,226 @@
+import SSA.Projects.RISCV.RV64
+import SSA.Projects.InstCombine.LLVM.Semantics
+import SSA.Projects.InstCombine.LLVM.PrettyEDSL
+import SSA.Projects.InstCombine.Refinement
+import SSA.Projects.InstCombine.Tactic
+import SSA.Projects.InstCombine.TacticAuto
+import SSA.Projects.InstCombine.Base
+import SSA.Projects.InstCombine.ForLean
+import Lean
+import Mathlib.Tactic.Ring
+import SSA.Projects.InstCombine.ForLean
+import SSA.Projects.InstCombine.LLVM.EDSL
+import SSA.Experimental.Bits.Fast.Reflect
+import SSA.Experimental.Bits.Fast.MBA
+import SSA.Experimental.Bits.FastCopy.Reflect
+import SSA.Experimental.Bits.AutoStructs.Tactic
+import SSA.Experimental.Bits.AutoStructs.ForLean
+import Std.Tactic.BVDecide
+import SSA.Core.Tactic.TacBench
+import Leanwuzla
+
+-- problems bc of registers
+-- proof of bitwise instruction wise translation via bit vec domain -> but with concrete input
+-- idea write a libary that translate each llvm instruction one to one into riscv instruction
+-- then lowert whole riscv into bit vec
+
+def ADD_RV64 :=
+  [RV64_com| {
+    ^entry (%X: !i64, %Y: !i64):
+    %v1 = "RV64.add" (%X, %Y) : (!i64, !i64) -> (!i64)
+    "return" (%v1) : (!i64, !i64) -> ()
+  }].denote
+
+def ADD_LLVM :=
+  [llvm(64)| {
+^bb0(%X : i64, %Y : i64):
+      %v1 = llvm.add %Y, %X : i64
+      llvm.return %v1 : i64
+  }].denote
+
+  def ADD_LLVM_BIG_CONTEXT :=
+    [llvm(64)| {
+^bb0(%X : i64, %Y : i64, %Z : i64, %W : i64):
+      %v1 = llvm.add %Y, %X : i64
+      llvm.return %v1 : i64
+  }]
+
+def lh_llvm : (HVector TyDenote.toType [InstCombine.Ty.bitvec 64,InstCombine.Ty.bitvec 64]) :=
+          HVector.cons (some (BitVec.ofNat 64 20)) <| HVector.cons (some (BitVec.ofNat 64 2)) .nil
+
+def lh_riscv : HVector TyDenote.toType [toRISCV.Ty.bv,toRISCV.Ty.bv ] :=
+  HVector.cons ((BitVec.ofNat 64 20)) <| HVector.cons ( (BitVec.ofNat 64 2)) .nil -- hvector from which we will create the valuation
+
+theorem translation_add_combined :
+    ADD_LLVM (Ctxt.Valuation.ofHVector lh_llvm) = some x →
+      x = ADD_RV64 (Ctxt.Valuation.ofHVector lh_riscv) := by
+    unfold ADD_RV64 lh_riscv ADD_LLVM lh_llvm
+    simp_alive_meta
+    simp_peephole [InstCombine.Op.denote,HVector.get,HVector.get, LLVM.add]
+    unfold RV64.RTYPE_pure64_RISCV_ADD
+    simp [HVector.cons_get_zero]
+    simp_alive_undef
+    intro h
+    injection h with h₁
+    rw [← h₁]
+    bv_decide
+
+def return_val_add : BitVec 64 := ADD_RV64 (Ctxt.Valuation.ofHVector lh_riscv)
+#eval return_val_add
+
+def OR_RV64 :=
+  [RV64_com| {
+    ^entry (%X: !i64, %Y: !i64):
+    %v1 = "RV64.add" (%X, %Y) : (!i64, !i64) -> (!i64)
+    "return" (%v1) : (!i64, !i64) -> ()
+  }].denote
+
+-- disjoint and normal or
+def OR_LLVM :=
+  [llvm(64)| {
+^bb0(%X : i64, %Y : i64):
+      %v1 = llvm.or %Y, %X : i64 -- handle disjoint flag
+      llvm.return %v1 : i64
+  }].denote
+
+def XOR_LLVM :=
+  [llvm(64)| {
+^bb0(%X : i64, %Y : i64):
+      %v1 = llvm.xor %Y, %X : i64
+      llvm.return %v1 : i64
+  }].denote
+
+def shl_LLVM :=
+  [llvm(64)| {
+^bb0(%X : i64, %Y : i64):
+      %v1 = llvm.shl %Y, %X : i64
+      llvm.return %v1 : i64
+  }].denote
+
+def shl_LLVM_flags :=
+  [llvm(64)| {
+^bb0(%X : i64, %Y : i64):
+      %v1 = llvm.add %Y, %X : i64
+      llvm.return %v1 : i64
+  }].denote
+
+--true and false flags
+def lshr_LLVM_ :=
+  [llvm(64)| {
+^bb0(%X : i64, %Y : i64):
+      %v1 = llvm.lshr %Y, %X : i64
+      llvm.return %v1 : i64
+  }].denote
+
+--true and false flags
+def ashr_LLVM_ :=
+  [llvm(64)| {
+^bb0(%X : i64, %Y : i64):
+      %v1 = llvm.ashr %Y, %X : i64
+      llvm.return %v1 : i64
+  }].denote
+
+def urem_LLVM_ :=
+  [llvm(64)| {
+^bb0(%X : i64, %Y : i64):
+      %v1 = llvm.urem %Y, %X : i64
+      llvm.return %v1 : i64
+  }].denote
+
+def srem_LLVM_ :=
+  [llvm(64)| {
+^bb0(%X : i64, %Y : i64):
+      %v1 = llvm.srem %Y, %X : i64
+      llvm.return %v1 : i64
+  }].denote
+
+def ADD_LLVM_flags :=
+  [llvm(64)| {
+^bb0(%X : i64, %Y : i64):
+      %v1 = llvm.add %Y, %X : i64
+      llvm.return %v1 : i64
+  }].denote
+
+def MUL_LLVM :=
+  [llvm(64)| {
+^bb0(%X : i64, %Y : i64):
+      %v1 = llvm.mul %Y, %X : i64
+      llvm.return %v1 : i64
+  }].denote
+
+def MUL_LLVM_flags :=
+  [llvm(64)| {
+^bb0(%X : i64, %Y : i64):
+      %v1 = llvm.add %Y, %X : i64
+      llvm.return %v1 : i64
+  }].denote
+
+
+def SUB_LLVM_ :=
+  [llvm(64)| {
+^bb0(%X : i64, %Y : i64):
+      %v1 = llvm.sub %Y, %X : i64
+      llvm.return %v1 : i64
+  }].denote
+
+
+def SUB_LLVM_flags :=
+  [llvm(64)| {
+^bb0(%X : i64, %Y : i64):
+      %v1 = llvm.add %Y, %X : i64
+      llvm.return %v1 : i64
+  }].denote
+
+-- true and false case
+def SDIV_LLVM_:=
+  [llvm(64)| {
+^bb0(%X : i64, %Y : i64):
+      %v1 = llvm.sdiv %Y, %X : i64
+      llvm.return %v1 : i64
+  }].denote
+
+-- true and false case
+def UDIV_LLVM_:=
+  [llvm(64)| {
+^bb0(%X : i64, %Y : i64):
+      %v1 = llvm.udiv %Y, %X : i64
+      llvm.return %v1 : i64
+  }].denote
+
+
+/-
+
+
+  | neg
+  | not
+  | copy
+  | trunc (w' : Width φ) (noWrapFlags : NoWrapFlags := {nsw := false, nuw := false} )
+  | zext  (w' : Width φ) (nneg : NonNegFlag := {nneg := false} )
+  | sext  (w' : Width φ)
+
+
+
+    | .and                => "and"
+    | .or   ⟨false⟩        => "or"
+    | .or   ⟨true⟩         => "or disjoint"
+    | .xor                => "xor"
+    | .shl  ⟨false, false⟩ => "shl"
+    | .shl  ⟨nsw, nuw⟩     => toString f!"shl {nsw} {nuw}"
+    | .lshr ⟨false⟩        => "lshr"
+    | .lshr ⟨true⟩         => "lshr exact"
+    | .ashr ⟨false⟩        => "ashr"
+    | .ashr ⟨true⟩         => "ashr exact"
+    | .urem               => "urem"
+    | .srem               => "srem"
+    | .add  ⟨false, false⟩ => "add"
+    | .add  ⟨nsw, nuw⟩     => toString f!"add {nsw} {nuw}"
+    | .mul  ⟨false, false⟩ => "mul"
+    | .mul  ⟨nsw, nuw⟩     => toString f!"mul {nsw} {nuw}"
+    | .sub  ⟨false, false⟩ => "sub"
+    | .sub  ⟨nsw, nuw⟩     => toString f!"sub {nsw} {nuw}"
+    | .sdiv ⟨false⟩        => "sdiv"
+    | .sdiv ⟨true⟩         => "sdiv exact"
+    | .udiv ⟨false⟩        => "udiv"
+    | .udiv ⟨true⟩         => "udiv exact"
+
+-/
